# 使用梯度下降法求解线性回归问题
+ 代价函数
$$J(\theta)=\frac{1}{2 \mathrm{m}} \sum_{i=1}^{m}\left(h_{\theta}\left(x^{(i)}\right)-y^{(i)}\right)^{2}$$
+ 求解
$$\begin{array}{l}
\frac{\partial}{\partial \theta_{j}} J(\theta)=\frac{\partial}{\partial \theta_{j}} \frac{1}{2 m} \sum_{i=1}^{m}\left(h_{\theta}\left(x^{(i)}\right)-y^{(i)}\right)^{2} \\
=2 * \frac{1}{2 m} \sum_{i=1}^{m}\left[\left(h_{\theta}\left(x^{(i)}\right)-y^{(i)}\right) \frac{\partial}{\partial \theta_{j}}\left(h_{\theta}\left(x^{(i)}\right)-y^{(i)}\right)\right] \\
=\frac{1}{m} \sum_{i=1}^{m}\left[\left(h_{\theta}\left(x^{(i)}\right)-y^{(i)}\right) \frac{\partial}{\partial \theta_{j}}\left(\sum_{f=0}^{n} \theta_{f} x_{f}^{(i)}-y^{(i)}\right)\right] \\
=\frac{1}{m} \sum_{i=1}^{m}\left[\left(h_{\theta}\left(x^{(i)}\right)-y^{(i)}\right) x_{j}^{(i)}\right] \\
\theta_{j}:=\theta_{j}+\alpha \frac{1}{m} \sum_{i=1}^{m}\left(y^{(i)}-h_{\theta}\left(x^{(i)}\right)\right) x_{j}^{(i)}
\end{array}$$
